TranslationCorrectness.v
@@ -897,7 +897,7 @@ Proof.
     econstructor; [now apply Hfindn|].
 
     inversion Hwdef as [|? ? Hwdef' neqs ni no
-                         Hwsch Hindi Hoivi Hnini Hndups Hfnone Hnname [HR1 HR2]].
+                         Hwsch Hindi Hoivi Hnini Hfnone Hnname [HR1 HR2]].
     unfold neqs,ni,no in *; clear neqs ni no HR1 HR2.
     simpl in *.
     clear Hfindn.
@@ -912,7 +912,7 @@ Proof.
       clear HR1 HR2 HR3 Hfindn.
     apply Memory_Corres_eqs_node_tl with (1:=Hord) (2:=Hnini) in Hmceqs.
 
-    clear Hwdef Hwsch Hindi Hoivi Hnini Hord Hndups.
+    clear Hwdef Hwsch Hindi Hoivi Hnini Hord.
     induction eqs as [|eq eqs IH]; [now constructor|].
     apply Forall_cons2 in Hmceqs.
     destruct Hmceqs as [Hmceq Hmceqs].
@@ -1662,8 +1662,7 @@ Proof.
   specialize Hi with n.
   specialize Ho with n.
 
-  inversion_clear Hwd as [|? ? Hwd' neqs ni no Hwsch Hin2
-                           Hout Hnode Hndups Hnd Hfind].
+  inversion_clear Hwd as [|? ? Hwd' neqs ni no Hwsch Hin2 Hout Hnode Hnd Hfind].
   rename Hwd' into Hwd.
   simpl in *.
   unfold neqs, ni, no in *; clear neqs ni no.
@@ -1877,8 +1876,7 @@ Proof.
       assert (Is_node_in g (eq::eqs)) as Hgini'.
       constructor 2; exact Hgini.
       now apply Hnin with (1:=Hgini'). }
-    pose proof (IHeqs Hmsems Hnin' Hnneq
-                      (Is_well_sch_cons _ _ _ Hwsch) _ _ Hevals)
+    pose proof (IHeqs Hmsems Hnin' (Is_well_sch_cons _ _ _ Hwsch) _ _ Hevals)
       as Hmc.
     clear IHeqs Hnin' Hmsems Hevals.
 
